theories/Examples/OperationalMulticoreProjectionExamples.v
@@ -1,0 +1,184 @@
+From Stdlib Require Import List Bool Arith Arith.PeanoNat Lia.
+From RocqSched Require Import Foundation.Base.
+From RocqSched Require Import Semantics.Schedule.
+From RocqSched Require Import Multicore.Common.MultiCoreBase.
+From RocqSched Require Import Multicore.Common.Admissibility.
+From RocqSched Require Import Multicore.Common.PlacementFacts.
+From RocqSched Require Import Multicore.Common.ValidityFacts.
+From RocqSched Require Import Operational.Common.State.
+From RocqSched Require Import Operational.Common.Invariants.
+From RocqSched Require Import Operational.Common.Projection.
+From RocqSched Require Import Operational.Common.Step.
+From RocqSched Require Import Operational.Common.Execution.
+From RocqSched Require Import Operational.Common.ProjectionLemmas.
+From RocqSched Require Import Operational.Common.ProjectionInvariants.
+From RocqSched Require Import Operational.Common.ProjectionMulticoreValidity.
+From RocqSched Require Import Operational.Awkernel.MinimalProjection.
+Import ListNotations.
+
+Section OperationalMulticoreProjectionExamples.
+
+  Definition mc_job0 : Job := mkJob 0 0 0 3 5.
+  Definition mc_job1 : Job := mkJob 1 0 0 2 4.
+
+  Definition mc_jobs (j : JobId) : Job :=
+    match j with
+    | 0 => mc_job0
+    | _ => mc_job1
+    end.
+
+  Definition even_odd_admissibility : admissible_cpu :=
+    fun j c => j = c.
+
+  Definition mc_running_state : OpState :=
+    mkOpState
+      (fun c =>
+         if Nat.eqb c 0 then Some 0
+         else if Nat.eqb c 1 then Some 1
+              else None)
+      []
+      (fun _ => false).
+
+  Definition mc_idle_state : OpState :=
+    mkOpState (fun _ => None) [] (fun _ => false).
+
+  Definition mc_trace (t : Time) : OpState :=
+    match t with
+    | 0 => mc_running_state
+    | _ => mc_idle_state
+    end.
+
+  Lemma mc_running_state_cpu_job :
+    forall c j,
+      c < 2 ->
+      op_current mc_running_state c = Some j ->
+      c = j.
+  Proof.
+    intros c j Hlt Hrun.
+    assert (Hc : c = 0 \/ c = 1) by lia.
+    destruct Hc as [-> | ->]; simpl in Hrun; inversion Hrun; subst; reflexivity.
+  Qed.
+
+  Lemma mc_trace_projectable :
+    projectable_trace mc_jobs 2 mc_trace.
+  Proof.
+    constructor.
+    - intros [|t'] j c1 c2 Hlt1 Hlt2 Hrun1 Hrun2.
+      + pose proof (mc_running_state_cpu_job c1 j Hlt1 Hrun1) as ->.
+        pose proof (mc_running_state_cpu_job c2 j Hlt2 Hrun2) as ->.
+        reflexivity.
+      + unfold mc_trace, mc_idle_state in Hrun1.
+        simpl in Hrun1.
+        discriminate.
+    - intros [|t'] c j Hlt Hrun.
+      + assert (Hcpu : c = 0 \/ c = 1) by lia.
+        destruct Hcpu as [-> | ->]; simpl in Hrun; inversion Hrun; subst;
+          unfold released, mc_jobs, mc_job0, mc_job1; simpl; lia.
+      + unfold mc_trace, mc_idle_state in Hrun.
+        simpl in Hrun.
+        discriminate.
+    - intros [|t'] c j Hlt Hrun.
+      + assert (Hcpu : c = 0 \/ c = 1) by lia.
+        destruct Hcpu as [-> | ->]; simpl in Hrun; inversion Hrun; subst;
+          unfold completed, service_job, cpu_count, runs_on, project_schedule,
+                 mc_trace, mc_running_state, mc_jobs, mc_job0, mc_job1; simpl; lia.
+      + unfold mc_trace, mc_idle_state in Hrun.
+        simpl in Hrun.
+        discriminate.
+  Qed.
+
+  Lemma mc_trace_idle_outside_range :
+    forall t, op_idle_outside_range 2 (mc_trace t).
+  Proof.
+    intros [|t'] c Hge.
+    - unfold mc_trace, mc_running_state.
+      simpl.
+      destruct (Nat.eqb c 0) eqn:Ec0.
+      + apply Nat.eqb_eq in Ec0. lia.
+      + destruct (Nat.eqb c 1) eqn:Ec1.
+        * apply Nat.eqb_eq in Ec1. lia.
+        * reflexivity.
+    - reflexivity.
+  Qed.
+
+  Lemma mc_trace_respects_admissibility :
+    forall t, op_respects_admissibility even_odd_admissibility 2 (mc_trace t).
+  Proof.
+    intros [|t'] c j Hlt Hrun.
+    - assert (Hcpu : c = 0 \/ c = 1) by lia.
+      destruct Hcpu as [-> | ->]; simpl in Hrun; inversion Hrun; subst;
+        unfold even_odd_admissibility; reflexivity.
+    - unfold mc_trace, mc_idle_state in Hrun.
+      simpl in Hrun.
+      discriminate.
+  Qed.
+
+  Example projected_schedule_respects_admissibility :
+    schedule_respects_admissibility even_odd_admissibility 2 (project_schedule mc_trace).
+  Proof.
+    apply op_respects_admissibility_projected.
+    exact mc_trace_respects_admissibility.
+  Qed.
+
+  Example projected_schedule_has_multicore_semantic_validity :
+    multicore_semantic_validity mc_jobs 2 (project_schedule mc_trace).
+  Proof.
+    apply projectable_trace_with_range_implies_multicore_semantic_validity.
+    - exact mc_trace_projectable.
+    - exact mc_trace_idle_outside_range.
+  Qed.
+
+  Definition awk_state : AwkernelState :=
+    mkAwkernelState (fun _ => None) [] (fun _ => false).
+
+  Definition awk_trace (_ : Time) : AwkernelState := awk_state.
+
+  Lemma awk_struct_inv :
+    forall t, op_struct_inv 2 (awk_to_op_state (awk_trace t)).
+  Proof.
+    intros t.
+    constructor.
+    - intros j c1 c2 Hlt1 Hlt2 Hrun1 Hrun2.
+      simpl in Hrun1.
+      discriminate.
+    - constructor.
+    - intros c j Hlt Hrun Hin.
+      simpl in Hin.
+      contradiction.
+  Qed.
+
+  Definition awk_execution_ex : awk_execution 2 :=
+    mkAwkExecution 2 awk_trace True (fun _ => ex_intro _ EvTick (step_tick _)) awk_struct_inv.
+
+  Lemma awk_execution_projection_sound :
+    awk_multicore_projection_sound mc_jobs even_odd_admissibility 2 awk_execution_ex.
+  Proof.
+    constructor.
+    - constructor.
+      + intros t c j Hlt Hrun.
+        unfold awk_trace, awk_state in Hrun.
+        simpl in Hrun.
+        discriminate.
+      + intros t c j Hlt Hrun.
+        unfold awk_trace, awk_state in Hrun.
+        simpl in Hrun.
+        discriminate.
+    - intros t.
+      unfold awk_trace, awk_state, awk_idle_outside_range, op_idle_outside_range.
+      intros c Hge.
+      reflexivity.
+    - intros t c j Hlt Hrun.
+      unfold awk_trace, awk_state, awk_respects_admissibility,
+             op_respects_admissibility, even_odd_admissibility in *.
+      simpl in Hrun.
+      discriminate.
+  Qed.
+
+  Example awk_projection_has_multicore_semantic_validity :
+    multicore_semantic_validity mc_jobs 2 (awk_project_schedule (awk_ex_trace awk_execution_ex)).
+  Proof.
+    eapply awk_multicore_projection_sound_implies_semantic_validity.
+    exact awk_execution_projection_sound.
+  Qed.
+
+End OperationalMulticoreProjectionExamples.
