theories/Operational/Common/ProjectionInvariants.v
@@ -1,0 +1,25 @@
+From Stdlib Require Import List Bool Arith Arith.PeanoNat Lia.
+From RocqSched Require Import Foundation.Base.
+From RocqSched Require Import Operational.Common.State.
+From RocqSched Require Import Operational.Common.Invariants.
+From RocqSched Require Import Multicore.Common.MultiCoreBase.
+
+Definition op_idle_outside_range (m : nat) (st : OpState) : Prop :=
+  forall c, m <= c -> op_current st c = None.
+
+Definition op_respects_admissibility
+    (adm : admissible_cpu) (m : nat) (st : OpState) : Prop :=
+  forall c j,
+    c < m ->
+    op_current st c = Some j ->
+    adm j c.
+
+Record op_multicore_projection_inv
+    (adm : admissible_cpu) (m : nat) (st : OpState) : Prop := {
+  ompi_struct :
+    op_struct_inv m st;
+  ompi_idle_outside :
+    op_idle_outside_range m st;
+  ompi_placement :
+    op_respects_admissibility adm m st;
+}.
