theories/Operational/Common/ProjectionMulticoreValidity.v
@@ -1,0 +1,117 @@
+From Stdlib Require Import List Bool Arith Arith.PeanoNat Lia.
+From RocqSched Require Import Foundation.Base.
+From RocqSched Require Import Semantics.Schedule.
+From RocqSched Require Import Multicore.Common.MultiCoreBase.
+From RocqSched Require Import Multicore.Common.Admissibility.
+From RocqSched Require Import Multicore.Common.PlacementFacts.
+From RocqSched Require Import Multicore.Common.ValidityFacts.
+From RocqSched Require Import Operational.Common.Trace.
+From RocqSched Require Import Operational.Common.Projection.
+From RocqSched Require Import Operational.Common.Execution.
+From RocqSched Require Import Operational.Common.ProjectionLemmas.
+From RocqSched Require Import Operational.Common.ProjectionInvariants.
+
+Lemma op_idle_outside_range_projected :
+  forall m tr,
+    (forall t, op_idle_outside_range m (tr t)) ->
+    forall t c,
+      m <= c ->
+      project_schedule tr t c = None.
+Proof.
+  intros m tr Hid t c Hge.
+  unfold project_schedule.
+  exact (Hid t c Hge).
+Qed.
+
+Lemma op_respects_admissibility_projected :
+  forall adm m tr,
+    (forall t, op_respects_admissibility adm m (tr t)) ->
+    schedule_respects_admissibility adm m (project_schedule tr).
+Proof.
+  intros adm m tr Hadm j t c Hlt Hrun.
+  unfold project_schedule in Hrun.
+  eapply Hadm; eauto.
+Qed.
+
+Lemma projectable_trace_implies_projected_no_duplication :
+  forall jobs m tr,
+    projectable_trace jobs m tr ->
+    no_duplication m (project_schedule tr).
+Proof.
+  intros jobs m tr Hproj.
+  apply op_no_duplication_implies_projected_no_duplication.
+  intro t.
+  exact (pt_no_dup _ _ _ Hproj t).
+Qed.
+
+Lemma projectable_trace_with_range_implies_multicore_semantic_validity :
+  forall jobs m tr,
+    projectable_trace jobs m tr ->
+    (forall t, op_idle_outside_range m (tr t)) ->
+    multicore_semantic_validity jobs m (project_schedule tr).
+Proof.
+  intros jobs m tr Hproj Hrange.
+  constructor.
+  - apply projectable_trace_implies_valid_schedule.
+    exact Hproj.
+  - apply projectable_trace_implies_projected_no_duplication with (jobs := jobs).
+    exact Hproj.
+  - apply op_idle_outside_range_projected.
+    exact Hrange.
+  - intros j t Hrunning.
+    unfold running_set_at in Hrunning.
+    destruct Hrunning as [c [Hlt Hrun]].
+    eapply projected_slot_eligible; eauto.
+Qed.
+
+Lemma projectable_trace_with_multicore_inv_implies_multicore_semantic_validity :
+  forall jobs adm m tr,
+    projectable_trace jobs m tr ->
+    (forall t, op_multicore_projection_inv adm m (tr t)) ->
+    multicore_semantic_validity jobs m (project_schedule tr) /\
+    schedule_respects_admissibility adm m (project_schedule tr).
+Proof.
+  intros jobs adm m tr Hproj Hinv.
+  split.
+  - apply projectable_trace_with_range_implies_multicore_semantic_validity; auto.
+    intro t.
+    exact (ompi_idle_outside _ _ _ (Hinv t)).
+  - apply op_respects_admissibility_projected.
+    intro t.
+    exact (ompi_placement _ _ _ (Hinv t)).
+Qed.
+
+Record execution_multicore_projection_sound
+    (jobs : JobId -> Job)
+    (adm : admissible_cpu)
+    (m : nat)
+    (ex : execution m) : Prop := {
+  emps_projection_sound :
+    execution_projection_sound jobs m ex;
+  emps_idle_outside :
+    forall t, op_idle_outside_range m (ex_trace ex t);
+  emps_placement :
+    forall t, op_respects_admissibility adm m (ex_trace ex t)
+}.
+
+Lemma execution_multicore_projection_sound_implies_semantic_validity :
+  forall jobs adm m ex,
+    execution_multicore_projection_sound jobs adm m ex ->
+    multicore_semantic_validity jobs m (project_schedule (ex_trace ex)).
+Proof.
+  intros jobs adm m ex Hsound.
+  eapply projectable_trace_with_range_implies_multicore_semantic_validity.
+  - apply execution_projection_sound_implies_projectable.
+    exact (emps_projection_sound _ _ _ _ Hsound).
+  - exact (emps_idle_outside _ _ _ _ Hsound).
+Qed.
+
+Lemma execution_multicore_projection_sound_implies_placement :
+  forall jobs adm m ex,
+    execution_multicore_projection_sound jobs adm m ex ->
+    schedule_respects_admissibility adm m (project_schedule (ex_trace ex)).
+Proof.
+  intros jobs adm m ex Hsound.
+  apply op_respects_admissibility_projected.
+  exact (emps_placement _ _ _ _ Hsound).
+Qed.
